list.dfy
@@ -1,29 +1,45 @@
 include "utils.dfy"
 include "Node.dfy"
 
+method INIT_LIST_HEAD(node: Node)
+  modifies node
+  ensures node.prev == node
+  ensures node.nodes == [node]
+  ensures node.next == node
+  ensures Singleton(node)
+{
+  node.prev := node;
+  node.next := node;
+  node.nodes := [node];
+}
 
 // analogue to __list_add
 method internal_list_add(new_node: Node, prev: Node, next: Node)
   requires Valid(new_node) && Valid(prev) && Valid(next) // must be valid nodes
+  requires prev.nodes[get_next_seq_idx(prev.nodes, IndexOf(prev.nodes, prev))] == next
+  requires same_linked_list([prev, next])
   requires Singleton(new_node) // must be a new node
   requires new_node != prev && new_node != next // all are different nodes
-  requires prev.nodes == next.nodes // same linked list
-  requires prev.next == next // next should be immediately after
-  modifies next, prev, new_node, multiset(prev.nodes)
+  modifies new_node, new_node.next, new_node.prev, multiset(prev.nodes)
   ensures Valid(new_node)
   ensures Valid(prev)
   ensures Valid(next)
   ensures same_linked_list([prev, next, new_node])
   ensures |prev.nodes| == |old(prev.nodes)|+1
   ensures (
-         var prev_idx := IndexOf(old(prev.nodes), prev);
-         && (prev_idx == |old(prev.nodes)|-1 ==> prev.nodes == old(prev.nodes) + [new_node])
-         && (0 <= prev_idx < |old(prev.nodes)|-1 ==> (
-           if |old(prev.nodes)| == 1 then prev.nodes == [prev, new_node]
-           else prev.nodes  == old(prev.nodes[..prev_idx])+[prev, new_node]+old(prev.nodes[(prev_idx+1)..]))
-         )
-       )
+            var prev_idx := IndexOf(old(prev.nodes), prev);
+            && (prev_idx == |old(prev.nodes)|-1 ==> prev.nodes == old(prev.nodes) + [new_node])
+            && (0 <= prev_idx < |old(prev.nodes)|-1 ==> (
+                    if |old(prev.nodes)| == 1 then prev.nodes == [prev, new_node]
+                    else prev.nodes  == old(prev.nodes[..prev_idx])+[prev, new_node]+old(prev.nodes[(prev_idx+1)..]))
+               )
+          )
+  ensures prev.nodes[get_next_seq_idx(prev.nodes, IndexOf(prev.nodes, prev))] == new_node
+  ensures prev.nodes[get_prev_seq_idx(prev.nodes, IndexOf(prev.nodes, next))] == new_node
 {
+  assert prev.next == next;
+  ghost var next_idx := IndexOf(prev.nodes, next);
+
   next.prev := new_node;
   new_node.next := next;
   new_node.prev := prev;
@@ -44,16 +60,40 @@ method internal_list_add(new_node: Node, prev: Node, next: Node)
       a'.nodes := new_nodes;
     }
   } else {
-    assert prev.nodes[prev_idx+1] == next;
-    ghost var new_nodes := [prev, new_node];
-    if |prev.nodes| > 1 {
-      assert prev.nodes[prev_idx+1] == next;
-      new_nodes := prev.nodes[..prev_idx] + [prev, new_node] + prev.nodes[(prev_idx+1)..];
+    assert 0 <= prev_idx < |prev.nodes|-1;
+    var splice_till_prev := prev.nodes[..prev_idx+1];
+    var splice_from_next := prev.nodes[next_idx..];
+    // var new_nodes := [];
+    if prev != next {
+      var new_nodes := splice_till_prev + [new_node] + splice_from_next;
+      assert prev_idx != next_idx;
+      assert prev_idx + 1 == next_idx;
+      assert Valid(prev) && Singleton(new_node) ==> forall node' :: node' in prev.nodes ==> node'.nodes == prev.nodes ==> new_node !in prev.nodes;
+      assert NoDupes(prev.nodes) ==> multiset(splice_till_prev) !! multiset(splice_from_next);
+      assert NoDupes(splice_till_prev);
+      assert NoDupes(splice_from_next);
+      assert new_node !in splice_till_prev && new_node !in splice_from_next ==> NoDupes(splice_till_prev + [new_node]+ splice_from_next) ==> NoDupes(new_nodes);
+
+      prev.nodes := new_nodes;
+      next.nodes := new_nodes;
+      new_node.nodes := new_nodes;
+      forall a' | a' in new_nodes {
+        a'.nodes := new_nodes;
+      }
+      // assert NoDupes(new_nodes) ==> NoDupes(new_node.nodes);
+    } else {
+      var new_nodes := splice_till_prev + [new_node];
+      assert Valid(prev) && Singleton(new_node) ==> forall node' :: node' in prev.nodes ==> node'.nodes == prev.nodes ==> new_node !in prev.nodes;
+      assert NoDupes(splice_till_prev);
+      assert new_node !in splice_till_prev ==> NoDupes(splice_till_prev + [new_node]) ==> NoDupes(new_nodes);
+
+      prev.nodes := new_nodes;
+      next.nodes := new_nodes;
+      new_node.nodes := new_nodes;
+      forall a' | a' in new_nodes {
+        a'.nodes := new_nodes;
+      }
     }
-    forall a' | a' in new_nodes {
-      a'.nodes := new_nodes;
-    }
-    assert prev in new_nodes && next in new_nodes && new_node in new_nodes;
   }
 }
 
@@ -69,6 +109,7 @@ method list_add(new_node: Node, head: Node)
   ensures head.nodes[get_next_seq_idx(head.nodes, IndexOf(head.nodes, head))] == new_node
 {
   assert head.nodes[(IndexOf(head.nodes, head)+1) % |head.nodes|] == head.next;
+  assert same_linked_list([head, head.next]);
   internal_list_add(new_node, head, head.next);
 }
 
@@ -83,12 +124,13 @@ method list_add_tail(new_node: Node, head: Node)
   ensures head.nodes[get_prev_seq_idx(head.nodes, IndexOf(head.nodes, head))] == new_node
 {
   assert head.nodes[(IndexOf(head.nodes, head)+|head.nodes|-1) % |head.nodes|] == head.prev;
+  assert same_linked_list([head, head.prev]);
   internal_list_add(new_node, head.prev, head);
 }
 
 ghost predicate same_linked_list(nodes: seq<Node>)
-requires |nodes| >= 1 
-reads multiset(nodes)
+  requires |nodes| >= 1
+  reads multiset(nodes)
 {
   var ghost_nodes := nodes[0].nodes;
   forall node' :: node' in nodes ==> node'.nodes == ghost_nodes
@@ -104,11 +146,11 @@ method internal_list_del(prev: Node, next: Node)
   ensures Valid(next)
   ensures same_linked_list([prev, next])
   ensures (
-    var idx := IndexOf(old(prev.nodes), prev);
-    && (idx == |old(prev.nodes)| - 1 ==> prev.nodes == old(prev.nodes[1..])) // prev is last, removed val is first index
-    && (idx == |old(prev.nodes)| - 2 ==> prev.nodes == old(prev.nodes[..|prev.nodes|-1])) // prev is second last, removed is the last element
-    && (0 <= idx < |old(prev.nodes)|-2 ==> prev.nodes == old(prev.nodes[..idx+1])+old(prev.nodes[idx+2..])) // anything else, then join arr till prev_idx] + [prev_idx+2..]
-  )
+            var idx := IndexOf(old(prev.nodes), prev);
+            && (idx == |old(prev.nodes)| - 1 ==> prev.nodes == old(prev.nodes[1..])) // prev is last, removed val is first index
+            && (idx == |old(prev.nodes)| - 2 ==> prev.nodes == old(prev.nodes[..|prev.nodes|-1])) // prev is second last, removed is the last element
+            && (0 <= idx < |old(prev.nodes)|-2 ==> prev.nodes == old(prev.nodes[..idx+1])+old(prev.nodes[idx+2..])) // anything else, then join arr till prev_idx] + [prev_idx+2..]
+          )
 {
   ghost var prev_idx := IndexOf(prev.nodes, prev);
   ghost var next_idx := IndexOf(prev.nodes, next);
@@ -132,7 +174,7 @@ method internal_list_del(prev: Node, next: Node)
     }
     assert prev.nodes[0] == next;
   } else if prev_idx == len - 2 {
-    assert prev_idx != |prev.nodes|-1; 
+    assert prev_idx != |prev.nodes|-1;
     assert prev_idx != |prev.nodes|-1;
     assert prev.nodes[0] == next;
     assert prev.nodes[|prev.nodes|-1] == prev_next;
@@ -142,7 +184,7 @@ method internal_list_del(prev: Node, next: Node)
       a'.nodes := new_nodes;
     }
   } else {
-    assert 0 <= prev_idx < |prev.nodes|-2; 
+    assert 0 <= prev_idx < |prev.nodes|-2;
     assert prev.nodes[prev_idx+1] == prev_next;
     assert prev.nodes[prev_idx+2] == next;
     assert next_idx == prev_idx+2;
@@ -160,27 +202,104 @@ method internal_list_del(prev: Node, next: Node)
 
 
 method list_del_entry(entry: Node)
-requires Valid(entry) 
-requires entry != entry.prev && entry != entry.next
-requires entry.next.nodes == entry.prev.nodes == entry.nodes
-modifies multiset(entry.nodes)
-ensures Valid(entry.prev)
-ensures Valid(entry.next)
+  requires Valid(entry)
+  requires entry != entry.prev && entry != entry.next
+  requires entry.next.nodes == entry.prev.nodes == entry.nodes
+  modifies multiset(entry.nodes)
+  ensures Valid(old(entry.prev))
+  ensures Valid(old(entry.next))
 {
-  var entry_next := entry.next;
-  var entry_prev := entry.prev;
-
   // assert entry != entry.prev && entry != entry.next  ==> |entry.nodes| >= 2;
   assert entry.nodes[get_prev_seq_idx(entry.nodes, IndexOf(entry.nodes, entry))] == entry.prev;
   assert entry.nodes[get_next_seq_idx(entry.nodes, IndexOf(entry.nodes, entry))] == entry.next;
-  
-  assert Valid(entry) && entry != entry.prev ==> |entry.nodes| >= 2;
-  // assert Valid(entry.prev) && Valid(entry) && entry.nodes == entry.prev.nodes ==> entry.prev.next == entry;
-  // assert Valid(entry.next) && Valid(entry) && entry.nodes == entry.next.nodes ==> entry.next.prev == entry;
-  // assert entry.prev.next.next == entry.next;
-  // assert entry.next.prev.prev == entry.prev;
+  internal_list_del(entry.prev, entry.next);
+}
 
-  internal_list_del(entry.prev, entry.next); 
+method list_replace(old_node: Node,
+                    new_node: Node)
+  requires Valid(old_node)
+  requires Valid(new_node)
+  requires old_node != new_node
+  requires Singleton(new_node)
+  requires new_node !in old_node.nodes
+  modifies new_node, old_node, old_node.next, new_node.next, new_node.prev, old_node.prev, multiset(old_node.nodes)
+  ensures Valid(new_node)
+  ensures (
+            var idx := IndexOf(old(old_node.nodes), old_node);
+            new_node.nodes == old(old_node.nodes[..idx]) + [new_node] + old(old_node.nodes[idx+1..])
+          )
+{
+  assert old_node.nodes[get_next_seq_idx(old_node.nodes, IndexOf(old_node.nodes, old_node))] == old_node.next;
+  assert old_node.nodes[get_prev_seq_idx(old_node.nodes, IndexOf(old_node.nodes, old_node))] == old_node.prev;
+  assert new_node !in old_node.nodes ==> old_node.next != new_node;
+  assert new_node !in old_node.nodes ==> old_node.prev != new_node;
 
-  assert |entry.prev.nodes| == |entry.nodes| - 1;
+  new_node.next := old_node.next;
+  new_node.next.prev := new_node;
+  new_node.prev := old_node.prev;
+  new_node.prev.next := new_node;
+
+
+  var old_idx := IndexOf(old_node.nodes, old_node);
+
+  assert new_node !in old_node.nodes;
+  var new_nodes := old_node.nodes[..old_idx] + [new_node]+ old_node.nodes[old_idx+1..];
+  assert |new_nodes| == |old_node.nodes|;
+  assert old_node !in new_nodes;
+  assert new_node in new_nodes;
+  assert new_node !in old_node.nodes[..old_idx] && new_node !in old_node.nodes[old_idx+1..];
+  assert NoDupes(old_node.nodes) ==> multiset(old_node.nodes[..old_idx]) !! multiset(old_node.nodes[old_idx+1..]);
+  assert NoDupes(old_node.nodes[..old_idx]);
+  assert NoDupes(old_node.nodes[old_idx+1..]);
+  assert NoDupes(old_node.nodes[..old_idx] + [new_node]+ old_node.nodes[old_idx+1..]);
+  new_node.nodes := new_nodes;
+  assert new_node.nodes[get_prev_seq_idx(new_nodes, IndexOf(new_node.nodes, new_node))] == new_node.prev;
+  assert old_node !in new_nodes;
+  forall a' | a' in new_nodes {
+    a'.nodes := new_nodes;
+  }
+}
+
+
+method list_replace_init(old_node: Node, new_node: Node)
+  requires Valid(old_node)
+  requires Valid(new_node)
+  requires !same_linked_list([old_node, new_node])
+  requires Singleton(new_node)
+  ensures Valid(new_node)
+  ensures Valid(old_node) && Singleton(old_node)
+  modifies new_node, old_node, old_node.next, new_node.next, new_node.prev, old_node.prev, multiset(old_node.nodes)
+{
+  // assert old_node != new_node && Singleton(new_node) ==> old_node !in new_node.nodes;
+  // assert Singleton(new_node) && Valid(old_node) ?==> new_node !in old_node.nodes;
+  list_replace(old_node, new_node);
+  INIT_LIST_HEAD(old_node);
+  assert Singleton(old_node) ==> Valid(old_node);
+}
+
+
+/**
+  * list_del_init - deletes entry from list and reinitialize it.
+  * @entry: the element to delete from the list.
+  */
+method list_del_init(entry: Node)
+  requires Valid(entry)
+  requires Valid(entry)
+  requires entry != entry.prev && entry != entry.next
+  requires entry.next.nodes == entry.prev.nodes == entry.nodes
+  modifies multiset(entry.nodes)
+  ensures Valid(entry) && Singleton(entry)
+{
+  assert entry.nodes[get_prev_seq_idx(entry.nodes, IndexOf(entry.nodes, entry))] == entry.prev;
+  assert entry.nodes[get_next_seq_idx(entry.nodes, IndexOf(entry.nodes, entry))] == entry.next;
+
+  ghost var entry_prev := entry.prev;
+  ghost var entry_next := entry.next;
+
+  list_del_entry(entry);
+
+  assert Valid(entry_prev);
+  assert Valid(entry_next);
+
+  INIT_LIST_HEAD(entry);
 }
